Given_Clause_Loops/Fair_Otter_Loop_Complete.thy
@@ -1,0 +1,92 @@
+(* Title:        Completeness of Fair Otter Loop
+   Authors:      Jasmin Blancherte <j.c.blanchette at vu.nl>, 2022
+   Maintainer:   Jasmin Blancherte <j.c.blanchette at vu.nl>, 2022
+*)
+
+section \<open>Completeness of Fair Otter Loop\<close>
+
+theory Fair_Otter_Loop_Complete
+  imports Fair_iProver_Loop
+begin
+
+
+(* FIXME *)
+
+subsection \<open>Completeness\<close>
+
+context fair_otter_loop
+begin
+
+theorem
+  assumes
+    olf_full: "full_chain (\<leadsto>OLf) Sts" and
+    olf_init: "is_initial_fair_OL_state (lhd Sts)" and
+    bot: "B \<in> Bot_F" and
+    unsat: "fset (new_of (lhd Sts)) \<Turnstile>\<inter>\<G> {B}"
+  shows
+    OL_complete_Liminf: "\<exists>B \<in> Bot_F. B \<in> state_union (Liminf_fstate Sts)" and
+    OL_complete: "\<exists>i. enat i < llength Sts \<and> (\<exists>B \<in> Bot_F. B \<in> all_of (lnth Sts i))"
+proof -
+  have ilf_chain: "chain (\<leadsto>ILf) Sts"
+    using Lazy_List_Chain.chain_mono fair_IL.ol full_chain_imp_chain olf_full by blast
+  hence ilf_full: "full_chain (\<leadsto>ILf) Sts"
+    by (metis chain_fair_IL_invariant_llast full_chain_iff_chain initial_fair_OL_invariant
+        is_final_fair_OL_state_iff_no_IL_step is_final_fair_OL_state_iff_no_OL_step olf_full
+        olf_init)
+
+  show "\<exists>B \<in> Bot_F. B \<in> state_union (Liminf_fstate Sts)"
+    by (rule IL_complete_Liminf[OF ilf_full olf_init bot unsat])
+  show "\<exists>i. enat i < llength Sts \<and> (\<exists>B \<in> Bot_F. B \<in> all_of (lnth Sts i))"
+    by (rule IL_complete[OF ilf_full olf_init bot unsat])
+qed
+
+end
+
+
+subsection \<open>Specialization with FIFO Queue\<close>
+
+locale fifo_otter_loop =
+  otter_loop Bot_F Inf_F Bot_G Q entails_q Inf_G_q Red_I_q Red_F_q \<G>_F_q \<G>_I_q Equiv_F Prec_F
+  for
+    Bot_F :: "'f set" and
+    Inf_F :: "'f inference set" and
+    Bot_G :: "'g set" and
+    Q :: "'q set" and
+    entails_q :: "'q \<Rightarrow> 'g set \<Rightarrow> 'g set \<Rightarrow> bool" and
+    Inf_G_q :: "'q \<Rightarrow> 'g inference set" and
+    Red_I_q :: "'q \<Rightarrow> 'g set \<Rightarrow> 'g inference set" and
+    Red_F_q :: "'q \<Rightarrow> 'g set \<Rightarrow> 'g set" and
+    \<G>_F_q :: "'q \<Rightarrow> 'f \<Rightarrow> 'g set" and
+    \<G>_I_q :: "'q \<Rightarrow> 'f inference \<Rightarrow> 'g inference set option" and
+    Equiv_F :: "'f \<Rightarrow> 'f \<Rightarrow> bool" (infix \<open>\<doteq>\<close> 50) and
+    Prec_F :: "'f \<Rightarrow> 'f \<Rightarrow> bool" (infix \<open>\<prec>\<cdot>\<close> 50) +
+  fixes
+    Prec_S :: "'f \<Rightarrow> 'f \<Rightarrow> bool" (infix "\<prec>S" 50)
+  assumes
+    wf_Prec_S: "minimal_element (\<prec>S) UNIV" and
+    transp_Prec_S: "transp (\<prec>S)" and
+    finite_Inf_between: "finite A \<Longrightarrow> finite (no_labels.Inf_between A {C})"
+begin
+
+sublocale fifo_passive_set
+  .
+
+sublocale fair_otter_loop Bot_F Inf_F Bot_G Q entails_q Inf_G_q Red_I_q Red_F_q \<G>_F_q \<G>_I_q
+  Equiv_F Prec_F "[]" hd "\<lambda>y xs. xs @ [y]" removeAll fset_of_list Prec_S
+proof unfold_locales
+  show "po_on (\<prec>S) UNIV"
+    using wf_Prec_S minimal_element.po by blast
+next
+  show "wfp_on (\<prec>S) UNIV"
+    using wf_Prec_S minimal_element.wf by blast
+next
+  show "transp (\<prec>S)"
+    by (rule transp_Prec_S)
+next
+  show "\<And>A C. finite A \<Longrightarrow> finite (no_labels.Inf_between A {C})"
+    by (fact finite_Inf_between)
+qed
+
+end
+
+end
